\ejercicio Calcular \begin{enumerate}[label=\roman*)] \item $\sumatoria{i=0}{n}2^i$\\
	      $ \sumatoria{i=0}{n}2^i \stackrel{q\neq1} = \frac{\red{2}^{n+1} - 1}{\red{2} - 1} = 2^{n+1} - 1 $

	\item $\sumatoria{i=1}{n} q^i$\\
	      $\sumatoria{i=1}{n} q^i = \red{-1 + 1} + \sumatoria{i=1}{n} q^i = \red{-1} + \sumatoria{i = \red{0}}{n} q^i =
		      \llave{lll}{
			      n + 1 \red{-1} = n & \text{si} & q = 1\\
			      \frac{q^{n+1}-1}{q-1} \red{-1} = \frac{q^{n+1} - q}{q-1} & \text{si} & q \distinto 1\\
		      }$

	\item \hacer
	\item \hacer
\end{enumerate}
