\ejercicio
$\flecha{del}[gr√°fico] (C \inter B) - A) \union (A - B) =\\
	\flecha{uso que}[$A - B = A \inter B^c$] = (C \inter B \inter A^c) \union (A \inter B^c) \stackrel{\blue{*}}{=}\\
	\flecha{distributiva} C \union (A \inter B^c) \inter B \union (A \inter B^c) \inter A^c \union (A \inter B^c) =\\
	= (C \union A) \inter (C \union B^c) \inter (B \union A) \inter (B \union B^c) \inter (A^c \union A) \inter (A^c \union B^c)=\\
	= (C \union A) \inter (C \union B^c) \inter (B \union A) \inter \universo \inter \universo \inter (A^c \union B^c)=\\
	= (C \union A) \inter (C \union B^c) \inter (B \union A) \inter (A^c \union B^c)=\\
	= C \inter C \union C \inter B^c \union A\inter C \union A \inter B^c ... \\
	= C \union C \inter B^c \union A\inter C \union A \inter B^c \\
$
