\ejercicio Sean $A$, $B$ y $C$ subconjuntos de un conjunto referencial $\universo$. Probar que:
\begin{enumerate}[label=\roman*)]
	\item $A \inter (B \triangle C) = (A \inter B) \triangle (A \inter C)$

	\item $A - (B - C) = (A-B) \union (A \inter C)$\\
	      $(A - B) \union (A \inter C) = A \inter [(A \inter B^c) \union C] = A \inter [(A \union C) \inter (B^c \union C)] =\\
		      A \inter (B^c \union C) = A \union(B-C)^c = A - (B - C)$

	\item $A \triangle B \subseteq (A \triangle C) \union (B \triangle C)$ \Hacer
	\item $(A \inter C ) - B = (A - B) \inter C$
	\item $A \subseteq B \entonces A \triangle B = B \inter A^c$
	\item $A \subseteq C \sisolosi B^c \subseteq A^c$
	\item $A \inter C = \vacio \entonces A \inter (B \triangle C) = A \inter B$
\end{enumerate}
